update the processor defs, still working on

model/agp32ProcessorScript.sml
@@ -35,233 +35,208 @@ End
 
 
 (* always_comb related *)
+(** assign instruction **)
+Definition IF_instr_update_def:
+  IF_instr_update fext (s:state_circuit) s' =
+  s' with IF := s'.IF with IF_instr := if fext.ready then fext.inst_rdata else 0x0000003Fw
+End
+   
 (** compute PC **)
 Definition IF_PC_sel_update_def:
-  IF_PC_sel_update (fext:ext) (s:state_circuit) s' =
-  if (s'.EX.EX_PC_sel = 1w) \/ ((s'.EX.EX_PC_sel = 2w) /\ (s'.EX.EX_ALU_res = 0w)) \/
-     ((s'.EX.EX_PC_sel = 3w) /\ (s'.EX.EX_ALU_res <> 0w)) then
-    s' with IF := s'.IF with PC_sel := s'.EX.EX_PC_sel
+  IF_PC_sel_update (fext:ext) s s' =
+  if (s.EX.EX_PC_sel = 1w) \/ ((s.EX.EX_PC_sel = 2w) /\ (s'.EX.EX_ALU_res = 0w)) \/
+     ((s.EX.EX_PC_sel = 3w) /\ (s'.EX.EX_ALU_res <> 0w)) then
+    s' with IF := s'.IF with PC_sel := s.EX.EX_PC_sel
   else s' with IF := s'.IF with PC_sel := 0w  
 End
    
 Definition IF_PC_input_update_def:
-  IF_PC_input_update (fext:ext) (s:state_circuit) s' =
+  IF_PC_input_update (fext:ext) s s' =
   s' with IF := s'.IF with
-                  IF_PC_input := MUX_41 s'.IF.PC_sel (s'.PC + 4w) s'.EX.EX_ALU_res
-                                        (s'.EX.EX_PC + s'.EX.EX_dataW_updated)
-                                        (s'.EX.EX_PC + s'.EX.EX_dataW_updated)
+                  IF_PC_input := MUX_41 s.IF.PC_sel (s.PC + 4w) s'.EX.EX_ALU_res
+                                        (s.EX.EX_PC + s.EX.EX_dataW_updated)
+                                        (s.EX.EX_PC + s.EX.EX_dataW_updated)
 End
 
 Theorem IF_PC_input_update_trans = REWRITE_RULE [MUX_41_def] IF_PC_input_update_def
 
-(** get register address from instr **)
-Definition ID_addr_update_def:
-  ID_addr_update (fext:ext) (s:state_circuit) s' =
-  let s' = s' with ID := s'.ID with ID_addrA := (22 >< 17) s'.ID.ID_instr;
-      s' = s' with ID := s'.ID with ID_addrB := (15 >< 10) s'.ID.ID_instr;
-      s' = s' with ID := s'.ID with ID_addrW := (30 >< 25) s'.ID.ID_instr;
-      s' = s' with ID := s'.ID with ID_addrA_enable := word_bit 23 s'.ID.ID_instr;
-      s' = s' with ID := s'.ID with ID_addrB_enable := word_bit 16 s'.ID.ID_instr in
-    s' with ID := s'.ID with ID_addrW_enable := word_bit 31 s'.ID.ID_instr
-End
-
 (** decode instr **)
-Definition ID_opc_update_def:
-  ID_opc_update (fext:ext) (s:state_circuit) s' =
-  if word_bit 24 s'.ID.ID_instr then
-    if word_bit 31 s'.ID.ID_instr then
-      s' with ID := s'.ID with ID_opc := 13w
-    else if (23 >< 9) s'.ID.ID_instr = 0w then
-      s' with ID := s'.ID with ID_opc := 14w
-    else
-      s' with ID := s'.ID with ID_opc := 15w
-  else if (5 >< 0) s'.ID.ID_instr = 10w \/ (5 >< 0) s'.ID.ID_instr = 11w \/
-          (5 >< 0) s'.ID.ID_instr = 12w then                                             
-    s' with ID := s'.ID with ID_opc := (5 >< 0) s'.ID.ID_instr
-  else if word_bit 31 s'.ID.ID_instr then
-    s' with ID := s'.ID with ID_opc := 15w
-  else if (5 >< 0) s'.ID.ID_instr <+ 10w then
-    s' with ID := s'.ID with ID_opc := (5 >< 0) s'.ID.ID_instr
-  else
-    s' with ID := s'.ID with ID_opc := 15w
-End
-
-Definition ID_func_update_def:
-  ID_func_update (fext:ext) (s:state_circuit) s' =
+Definition ID_opc_func_update_def:
+  ID_opc_func_update (fext:ext) s s' =
+  let s' = if word_bit 24 s.ID.ID_instr then
+             if word_bit 31 s.ID.ID_instr then
+               s' with ID := s'.ID with ID_opc := 13w
+             else if (23 >< 9) s.ID.ID_instr = 0w then
+               s' with ID := s'.ID with ID_opc := 14w
+             else
+               s' with ID := s'.ID with ID_opc := 15w
+           else if (5 >< 0) s.ID.ID_instr = 10w \/ (5 >< 0) s.ID.ID_instr = 11w \/
+                   (5 >< 0) s.ID.ID_instr = 12w then                                             
+             s' with ID := s'.ID with ID_opc := (5 >< 0) s.ID.ID_instr
+           else if word_bit 31 s.ID.ID_instr then
+             s' with ID := s'.ID with ID_opc := 15w
+           else if (5 >< 0) s.ID.ID_instr <+ 10w then
+             s' with ID := s'.ID with ID_opc := (5 >< 0) s.ID.ID_instr
+           else
+             s' with ID := s'.ID with ID_opc := 15w in
   if s'.ID.ID_opc = 0w \/ s'.ID.ID_opc = 1w \/ s'.ID.ID_opc = 6w \/
      s'.ID.ID_opc = 9w \/ s'.ID.ID_opc = 10w \/ s'.ID.ID_opc = 11w then
-    s' with ID := s'.ID with ID_func := (9 >< 6) s'.ID.ID_instr
+    s' with ID := s'.ID with ID_func := (9 >< 6) s.ID.ID_instr
   else
     s' with ID := s'.ID with ID_func := 9w
 End
 
-(** register read **)
-Definition REG_read_def:
-  REG_read (fext:ext) (s:state_circuit) s' =
-  let s' = s' with ID := s'.ID with ID_read_dataA := s'.R s'.ID.ID_addrA;
-      s' = s' with ID := s'.ID with ID_read_dataB := s'.R s'.ID.ID_addrB in
-    s' with ID := s'.ID with ID_read_dataW := s'.R s'.ID.ID_addrW
-End
-
-(** generate immediate **)
-Definition ID_imm_update_def:
-  ID_imm_update (fext:ext) (s:state_circuit) s' =
-  if word_bit 31 s'.ID.ID_instr /\ word_bit 24 s'.ID.ID_instr then
-    if word_bit 23 s'.ID.ID_instr then
-      s' with ID := s'.ID with ID_imm := 0w - w2w ((22 >< 0) s'.ID.ID_instr)
-    else
-      s' with ID := s'.ID with ID_imm := w2w ((22 >< 0) s'.ID.ID_instr)
-  else if word_bit 24 s'.ID.ID_instr /\ (23 >< 9) s'.ID.ID_instr = 0w then
-    s' with ID := s'.ID with ID_imm := w2w ((8 >< 0) s'.ID.ID_instr)
-  else
-    s' with ID := s'.ID with ID_imm := 0w
-End
-
-Definition ID_imm_reg_update_def:
-  ID_imm_reg_update (fext:ext) (s:state_circuit) s' =
-  let s' = s' with ID := s'.ID with ID_immA := sw2sw ((22 >< 17) s'.ID.ID_instr);
-      s' = s' with ID := s'.ID with ID_immB := sw2sw ((15 >< 10) s'.ID.ID_instr) in
-    s' with ID := s'.ID with ID_immW := sw2sw ((30 >< 25) s'.ID.ID_instr)
-End
-
-(** update the value from reg in case the addr is written by the WB stage **)
-Definition ID_forward_update_def:
-  ID_forward_update (fext:ext) (s:state_circuit) s' =
-  let s' = s' with ID := s'.ID with ID_ForwardA := if s'.ID.ID_addrA = s'.WB.WB_addrW /\
-                                                      s'.WB.WB_write_reg /\ s'.WB.WB_state_flag then T
-                                                   else F;
-      s' = s' with ID := s'.ID with ID_ForwardB := if s'.ID.ID_addrB = s'.WB.WB_addrW /\
-                                                      s'.WB.WB_write_reg /\ s'.WB.WB_state_flag then T
-                                                   else F in
-    s' with ID := s'.ID with ID_ForwardW := if s'.ID.ID_addrW = s'.WB.WB_addrW /\
-                                               s'.WB.WB_write_reg /\ s'.WB.WB_state_flag then T
-                                            else F
-End
-    
-Definition ID_read_data_update_def:
-  ID_read_data_update (fext:ext) (s:state_circuit) s' =
-  let s' = s' with ID := s'.ID with ID_read_dataA_updated :=
-           MUX_21 s'.ID.ID_ForwardA s'.ID.ID_read_dataA s'.WB.WB_write_data;
-      s' = s' with ID := s'.ID with ID_read_dataB_updated :=
-           MUX_21 s'.ID.ID_ForwardB s'.ID.ID_read_dataB s'.WB.WB_write_data in
-  s' with ID := s'.ID with ID_read_dataW_updated :=
-  MUX_21 s'.ID.ID_ForwardW s'.ID.ID_read_dataW s'.WB.WB_write_data
-End
-
-Theorem ID_read_data_update_trans = REWRITE_RULE [MUX_21_def] ID_read_data_update_def
-
 (** update the data from read_data and imm for A/B/W **)
 Definition ID_data_update_def:
-  ID_data_update (fext:ext) (s:state_circuit) s' =
-  let s' = s' with ID := s'.ID with ID_dataA :=
-           MUX_21 (word_bit 23 s'.ID.ID_instr) s'.ID.ID_read_dataA_updated s'.ID.ID_immA;
+  ID_data_update (fext:ext) s s' =
+  let s' = s' with ID := s'.ID with ID_addrA := (22 >< 17) s.ID.ID_instr;
+      s' = s' with ID := s'.ID with ID_addrB := (15 >< 10) s.ID.ID_instr;
+      s' = s' with ID := s'.ID with ID_addrW := (30 >< 25) s.ID.ID_instr;
+      s' = s' with ID := s'.ID with ID_addrA_enable := word_bit 23 s.ID.ID_instr;
+      s' = s' with ID := s'.ID with ID_addrB_enable := word_bit 16 s.ID.ID_instr;
+      s' = s' with ID := s'.ID with ID_addrW_enable := word_bit 31 s.ID.ID_instr;
+      s' = s' with ID := s'.ID with ID_read_dataA := s'.R s'.ID.ID_addrA;
+      s' = s' with ID := s'.ID with ID_read_dataB := s'.R s'.ID.ID_addrB;
+      s' = s' with ID := s'.ID with ID_read_dataW := s'.R s'.ID.ID_addrW;
+      s' = s' with ID := s'.ID with ID_immA := sw2sw ((22 >< 17) s.ID.ID_instr);
+      s' = s' with ID := s'.ID with ID_immB := sw2sw ((15 >< 10) s.ID.ID_instr);
+      s' = s' with ID := s'.ID with ID_immW := sw2sw ((30 >< 25) s.ID.ID_instr);
+      s' = s' with ID := s'.ID with ID_ForwardA := if s'.ID.ID_addrA = s.WB.WB_addrW /\
+                                                      s.WB.WB_write_reg /\ s.WB.WB_state_flag then T
+                                                   else F;
+      s' = s' with ID := s'.ID with ID_ForwardB := if s'.ID.ID_addrB = s.WB.WB_addrW /\
+                                                      s.WB.WB_write_reg /\ s.WB.WB_state_flag then T
+                                                   else F;
+      s' = s' with ID := s'.ID with ID_ForwardW := if s'.ID.ID_addrW = s.WB.WB_addrW /\
+                                                      s.WB.WB_write_reg /\ s.WB.WB_state_flag then T
+                                                   else F;
+      s' = s' with ID := s'.ID with ID_read_dataA_updated :=
+           MUX_21 s'.ID.ID_ForwardA s'.ID.ID_read_dataA s.WB.WB_write_data;
+      s' = s' with ID := s'.ID with ID_read_dataB_updated :=
+           MUX_21 s'.ID.ID_ForwardB s'.ID.ID_read_dataB s.WB.WB_write_data;
+      s' = s' with ID := s'.ID with ID_read_dataW_updated :=
+           MUX_21 s'.ID.ID_ForwardW s'.ID.ID_read_dataW s.WB.WB_write_data;
+      s' = s' with ID := s'.ID with ID_dataA :=
+           MUX_21 (word_bit 23 s.ID.ID_instr) s'.ID.ID_read_dataA_updated s'.ID.ID_immA;
       s' = s' with ID := s'.ID with ID_dataB :=
-           MUX_21 (word_bit 16 s'.ID.ID_instr) s'.ID.ID_read_dataB_updated s'.ID.ID_immB in
+           MUX_21 (word_bit 16 s.ID.ID_instr) s'.ID.ID_read_dataB_updated s'.ID.ID_immB in
     s' with ID := s'.ID with ID_dataW :=
-    MUX_21 (word_bit 31 s'.ID.ID_instr) s'.ID.ID_read_dataW_updated s'.ID.ID_immW
+    MUX_21 (word_bit 31 s.ID.ID_instr) s'.ID.ID_read_dataW_updated s'.ID.ID_immW
 End
 
 Theorem ID_data_update_trans = REWRITE_RULE [MUX_21_def] ID_data_update_def
 
+(** generate immediate **)
+Definition ID_imm_update_def:
+  ID_imm_update (fext:ext) s s' =
+  if word_bit 31 s.ID.ID_instr /\ word_bit 24 s.ID.ID_instr then
+    if word_bit 23 s.ID.ID_instr then
+      s' with ID := s'.ID with ID_imm := 0w - w2w ((22 >< 0) s.ID.ID_instr)
+    else
+      s' with ID := s'.ID with ID_imm := w2w ((22 >< 0) s.ID.ID_instr)
+  else if word_bit 24 s.ID.ID_instr /\ (23 >< 9) s.ID.ID_instr = 0w then
+    s' with ID := s'.ID with ID_imm := w2w ((8 >< 0) s.ID.ID_instr)
+  else
+    s' with ID := s'.ID with ID_imm := 0w
+End
+
 (** set up flags of EX stage **)
 Definition EX_ctrl_update_def:
-  EX_ctrl_update (fext:ext) (s:state_circuit) s' =
-  if s'.ID.ID_EX_write_enable then
-    s' with EX := s'.EX with EX_isAcc := (s'.EX.EX_opc = 8w)
+  EX_ctrl_update (fext:ext) s s' =
+  if s.ID.ID_EX_write_enable then
+    let s' = s' with EX := s'.EX with EX_isAcc := (s.EX.EX_opc = 8w) in
+      s' with EX := s'.EX with EX_PC_sel := if s.EX.EX_opc = 9w then 1w
+                                            else if s.EX.EX_opc = 10w then 2w
+                                            else if s.EX.EX_opc = 11w then 3w
+                                            else 0w
   else s'
 End
 
 (** forward data from MEM/WB -> EX **)
 Definition EX_forward_data_def:
-  EX_forward_data (fext:ext) (s:state_circuit) s' =
+  EX_forward_data (fext:ext) s s' =
   let s' = s' with EX := s'.EX with EX_dataA_updated :=
-           MUX_81 s'.EX.EX_ForwardA s'.EX.EX_dataA s'.WB.WB_write_data
-                  s'.MEM.MEM_ALU_res s'.MEM.MEM_SHIFT_res
-                  (s'.MEM.MEM_PC + 4w) s'.MEM.MEM_imm_updated 0w 0w;
+           MUX_81 s.EX.EX_ForwardA s'.EX.EX_dataA s.WB.WB_write_data
+                  s.MEM.MEM_ALU_res s.MEM.MEM_SHIFT_res
+                  (s.MEM.MEM_PC + 4w) s.MEM.MEM_imm_updated 0w 0w;
      s' = s' with EX := s'.EX with EX_dataB_updated :=
-          MUX_81 s'.EX.EX_ForwardB s'.EX.EX_dataB s'.WB.WB_write_data
-                 s'.MEM.MEM_ALU_res s'.MEM.MEM_SHIFT_res
-                 (s'.MEM.MEM_PC + 4w) s'.MEM.MEM_imm_updated 0w 0w in
+          MUX_81 s.EX.EX_ForwardB s'.EX.EX_dataB s.WB.WB_write_data
+                 s.MEM.MEM_ALU_res s.MEM.MEM_SHIFT_res
+                 (s.MEM.MEM_PC + 4w) s.MEM.MEM_imm_updated 0w 0w in
     s' with EX := s'.EX with EX_dataW_updated :=
-    MUX_81 s'.EX.EX_ForwardW s'.EX.EX_dataW s'.WB.WB_write_data
-           s'.MEM.MEM_ALU_res s'.MEM.MEM_SHIFT_res
-           (s'.MEM.MEM_PC + 4w) s'.MEM.MEM_imm_updated 0w 0w
+    MUX_81 s.EX.EX_ForwardW s'.EX.EX_dataW s.WB.WB_write_data
+           s.MEM.MEM_ALU_res s.MEM.MEM_SHIFT_res
+           (s.MEM.MEM_PC + 4w) s.MEM.MEM_imm_updated 0w 0w
 End
 
 Theorem EX_forward_data_trans = REWRITE_RULE [MUX_81_def] EX_forward_data_def
 
 (** set up inputs for ALU **)
 Definition EX_ALU_input_update_def:
-  EX_ALU_input_update (fext:ext) (s:state_circuit) s' =
+  EX_ALU_input_update (fext:ext) s s' =
   let s' = s' with EX := s'.EX with EX_ALU_input1 :=
-           MUX_21 (s'.EX.EX_opc = 9w) s'.EX.EX_dataA_updated s'.EX.EX_PC in
+           MUX_21 (s.EX.EX_opc = 9w) s.EX.EX_dataA_updated s.EX.EX_PC in
     s' with EX := s'.EX with EX_ALU_input2 :=
-    MUX_21 (s'.EX.EX_opc = 9w) s'.EX.EX_dataB_updated s'.EX.EX_dataA_updated
+    MUX_21 (s.EX.EX_opc = 9w) s.EX.EX_dataB_updated s.EX.EX_dataA_updated
 End
 
 Theorem EX_ALU_input_update_trans = REWRITE_RULE [MUX_21_def] EX_ALU_input_update_def
 
 (** EX_compute_enable: aviod errors due to stalling **)
 Definition EX_compute_enable_update_def:
-  EX_compute_enable_update (fext:ext) (s:state_circuit) s' =
+  EX_compute_enable_update (fext:ext) s s' =
   s' with EX := s'.EX with EX_compute_enable := (s'.state = 0w /\
-                                                (s'.MEM.MEM_opc <> 16w \/ s'.MEM.MEM_opc = 16w /\
-                                                (s'.EX.EX_ForwardA <> 0w \/ s'.EX.EX_ForwardB <> 0w)))
+                                                (s.MEM.MEM_opc <> 16w \/ (s.MEM.MEM_opc = 16w /\
+                                                (s.EX.EX_ForwardA <> 0w \/ s.EX.EX_ForwardB <> 0w))))
 End
 
 (** ALU **)
 Definition EX_ALU_update_def:
-  EX_ALU_update (fext:ext) (s:state_circuit) s' =
-  let input1 = s'.EX.EX_ALU_input1;
-      input2 = s'.EX.EX_ALU_input2;
-      func = s'.EX.EX_func;
-      ALU_sum = (w2w input1 + w2w input2 +
-                 (if func = 1w then v2w [s'.EX.EX_carry_flag] else 0w)) : 33 word;
-      ALU_prod = (w2w input1 * w2w input2) : word64 in
-  if s'.EX.EX_compute_enable then
-    case func of
-      0w => let s' = s' with EX := s'.EX with EX_overflow_flag :=
-                    ((word_bit 31 input1 = word_bit 31 input2) /\
-                     (word_bit 31 ALU_sum <> word_bit 31 input1));
-                s' = s' with EX := s'.EX with EX_carry_flag := word_bit 32 ALU_sum in
-              s' with EX := s'.EX with EX_ALU_res := (31 >< 0) ALU_sum
-    | 1w => let s' = s' with EX := s'.EX with EX_carry_flag := word_bit 32 ALU_sum in
-              s' with EX := s'.EX with EX_ALU_res := (31 >< 0) ALU_sum
-    | 2w => let ALU_sub = input1 − input2;
-                s' = s' with EX := s'.EX with EX_ALU_res := ALU_sub in
-              s' with EX := s'.EX with EX_overflow_flag := ((word_bit 31 input1 <> word_bit 31 input2) /\
-                                                          (word_bit 31 ALU_sub <> word_bit 31 input1))
+  EX_ALU_update (fext:ext) s s' =
+  let s' = s' with ALU_sum := (w2w s.EX.EX_ALU_input1 + w2w s.EX.EX_ALU_input2 +
+                              (if s'.EX.EX_func = 1w then v2w [s'.EX.EX_carry_flag] else 0w));
+      s' = s' with ALU_prod := (w2w s.EX.EX_ALU_input1 * w2w s.EX.EX_ALU_input2) in
+  if s.EX.EX_compute_enable then
+    case s'.EX.EX_func of
+      0w => (let s' = s' with EX := s'.EX with EX_overflow_flag :=
+                      ((word_bit 31 s.EX.EX_ALU_input1 = word_bit 31 s.EX.EX_ALU_input2) /\
+                       (word_bit 31 s'.ALU_sum <> word_bit 31 s.EX.EX_ALU_input1));
+                 s' = s' with EX := s'.EX with EX_carry_flag := word_bit 32 s'.ALU_sum in
+               s' with EX := s'.EX with EX_ALU_res := (31 >< 0) s'.ALU_sum)
+    | 1w => (let s' = s' with EX := s'.EX with EX_carry_flag := word_bit 32 s'.ALU_sum in
+               s' with EX := s'.EX with EX_ALU_res := (31 >< 0) s'.ALU_sum)
+    | 2w => (let s' = s' with ALU_sub := s.EX.EX_ALU_input1 − s.EX.EX_ALU_input2;
+                 s' = s' with EX := s'.EX with EX_ALU_res := s'.ALU_sub in
+               s' with EX := s'.EX with EX_overflow_flag :=
+               ((word_bit 31 s.EX.EX_ALU_input1 <> word_bit 31 s.EX.EX_ALU_input2) /\
+                (word_bit 31 s'.ALU_sub <> word_bit 31 s.EX.EX_ALU_input1)))
     | 3w => s' with EX := s'.EX with EX_ALU_res := v2w [s'.EX.EX_carry_flag]
     | 4w => s' with EX := s'.EX with EX_ALU_res := v2w [s'.EX.EX_overflow_flag]
-    | 5w => s' with EX := s'.EX with EX_ALU_res := input1 + 1w
-    | 6w => s' with EX := s'.EX with EX_ALU_res := input1 - 1w
-    | 7w => s' with EX := s'.EX with EX_ALU_res := (31 >< 0) ALU_prod
-    | 8w => s' with EX := s'.EX with EX_ALU_res := (63 >< 32) ALU_prod
-    | 9w => s' with EX := s'.EX with EX_ALU_res := (input1 && input2)
-    | 10w => s' with EX := s'.EX with EX_ALU_res := (input1 || input2)
-    | 11w => s' with EX := s'.EX with EX_ALU_res := (input1 ?? input2)
-    | 12w => s' with EX := s'.EX with EX_ALU_res := v2w [input1 = input2]
-    | 13w => s' with EX := s'.EX with EX_ALU_res := v2w [input1 < input2]
-    | 14w => s' with EX := s'.EX with EX_ALU_res := v2w [input1 <+ input2]
-    | 15w => s' with EX := s'.EX with EX_ALU_res := input2
+    | 5w => s' with EX := s'.EX with EX_ALU_res := s.EX.EX_ALU_input1 + 1w
+    | 6w => s' with EX := s'.EX with EX_ALU_res := s.EX.EX_ALU_input1 - 1w
+    | 7w => s' with EX := s'.EX with EX_ALU_res := (31 >< 0) s'.ALU_prod
+    | 8w => s' with EX := s'.EX with EX_ALU_res := (63 >< 32) s'.ALU_prod
+    | 9w => s' with EX := s'.EX with EX_ALU_res := (s.EX.EX_ALU_input1 && s.EX.EX_ALU_input2)
+    | 10w => s' with EX := s'.EX with EX_ALU_res := (s.EX.EX_ALU_input1 || s.EX.EX_ALU_input2)
+    | 11w => s' with EX := s'.EX with EX_ALU_res := (s.EX.EX_ALU_input1 ?? s.EX.EX_ALU_input2)
+    | 12w => s' with EX := s'.EX with EX_ALU_res := v2w [s.EX.EX_ALU_input1 = s.EX.EX_ALU_input2]
+    | 13w => s' with EX := s'.EX with EX_ALU_res := v2w [s.EX.EX_ALU_input1 < s.EX.EX_ALU_input2]
+    | 14w => s' with EX := s'.EX with EX_ALU_res := v2w [s.EX.EX_ALU_input1 <+ s.EX.EX_ALU_input2]
+    | 15w => s' with EX := s'.EX with EX_ALU_res := s.EX.EX_ALU_input2
   else s'
 End
 
 (** SHIFT **)
-Definition SHIFT_def:
-  SHIFT (func:word2) inputa inputb s =
-  case func of
-     0w => s with EX := s.EX with EX_SHIFT_res := inputa <<~ inputb
-   | 1w => s with EX := s.EX with EX_SHIFT_res := inputa >>>~ inputb
-   | 2w => s with EX := s.EX with EX_SHIFT_res := inputa >>~ inputb
-   | 3w => let shift_sh = word_mod inputb 32w in
-             s with EX := s.EX with EX_SHIFT_res := (inputa >>>~ shift_sh) || (inputa <<~ (32w - shift_sh))
-End
-
 Definition EX_SHIFT_update_def:
-  EX_SHIFT_update (fext:ext) (s:state_circuit) s' =
-  if s'.EX.EX_compute_enable then
-    SHIFT ((1 >< 0) s'.EX.EX_func) s'.EX.EX_dataA_updated s'.EX.EX_dataB_updated s'
+  EX_SHIFT_update (fext:ext) s s' =
+  if s.EX.EX_compute_enable then
+    case ((1 >< 0) s'.EX.EX_func) of
+      0w => s' with EX := s'.EX with EX_SHIFT_res := s.EX.EX_dataA_updated <<~ s.EX.EX_dataB_updated
+    | 1w => s' with EX := s'.EX with EX_SHIFT_res := s.EX.EX_dataA_updated >>>~ s.EX.EX_dataB_updated
+    | 2w => s' with EX := s'.EX with EX_SHIFT_res := s.EX.EX_dataA_updated >>~ s.EX.EX_dataB_updated
+    | 3w => let s' = s' with shift_sh := word_mod s.EX.EX_dataB_updated 32w in
+              s' with EX := s'.EX with EX_SHIFT_res :=
+              (s.EX.EX_dataA_updated >>>~ s'.shift_sh) || (s.EX.EX_dataA_updated <<~ (32w - s'.shift_sh))
   else s'
 End
 
@@ -271,98 +246,82 @@ Proof
  gen_tac >> CONV_TAC (LHS_CONV wordsLib.WORD_MOD_BITS_CONV) >> blastLib.BBLAST_TAC
 QED
 
-Theorem EX_SHIFT_update_trans = REWRITE_RULE [SHIFT_def,word_mod_32] EX_SHIFT_update_def
+Theorem EX_SHIFT_update_trans = REWRITE_RULE [word_mod_32] EX_SHIFT_update_def
 
 (** record data **)
 Definition EX_data_rec_update_def:
   EX_data_rec_update (fext:ext) (s:state_circuit) s' =
-  if s'.state = 0w /\ s'.MEM.MEM_opc <> 16w then
-    let s' = s' with EX := s'.EX with EX_dataA_rec := s'.EX.EX_dataA_updated;
-        s' = s' with EX := s'.EX with EX_dataB_rec := s'.EX.EX_dataB_updated in
-      s' with EX := s'.EX with EX_dataW_rec := s'.EX.EX_dataW_updated
-  else if s'.state = 0w /\ s'.MEM.MEM_opc = 16w then
+  if s'.state = 0w /\ s.MEM.MEM_opc <> 16w then
+    let s' = s' with EX := s'.EX with EX_dataA_rec := s.EX.EX_dataA_updated;
+        s' = s' with EX := s'.EX with EX_dataB_rec := s.EX.EX_dataB_updated in
+      s' with EX := s'.EX with EX_dataW_rec := s.EX.EX_dataW_updated
+  else if s'.state = 0w /\ s.MEM.MEM_opc = 16w then
     let s' = s' with EX := s'.EX with EX_dataA_rec :=
-             if s'.EX.EX_ForwardA <> 0w then s'.EX.EX_dataA_updated
+             if s.EX.EX_ForwardA <> 0w then s.EX.EX_dataA_updated
              else s'.EX.EX_dataA_rec;
         s' = s' with EX := s'.EX with EX_dataB_rec :=
-             if s'.EX.EX_ForwardB <> 0w then s'.EX.EX_dataB_updated
+             if s.EX.EX_ForwardB <> 0w then s.EX.EX_dataB_updated
              else s'.EX.EX_dataB_rec in
       s' with EX := s'.EX with EX_dataW_rec :=
-      if s'.EX.EX_ForwardW <> 0w then s'.EX.EX_dataW_updated
+      if s.EX.EX_ForwardW <> 0w then s.EX.EX_dataW_updated
       else s'.EX.EX_dataW_rec
   else s'
 End
 
 (** Set up flags of MEM stage **)
 Definition MEM_ctrl_update_def:
-  MEM_ctrl_update (fext:ext) (s:state_circuit) s' =
-  if (s'.EX.EX_write_enable /\ s'.MEM.MEM_state_flag) \/ s'.MEM.MEM_enable then
-    let s' = s' with MEM := s'.MEM with MEM_read_mem := (s'.MEM.MEM_opc = 4w \/ s'.MEM.MEM_opc = 5w);
-        s' = s' with MEM := s'.MEM with MEM_write_mem := (s'.MEM.MEM_opc = 2w);
-        s' = s' with MEM := s'.MEM with MEM_write_mem_byte := (s'.MEM.MEM_opc = 3w);
-        s' = s' with MEM := s'.MEM with MEM_write_reg := (s'.MEM.MEM_opc = 0w \/ s'.MEM.MEM_opc = 1w \/
-                                                          s'.MEM.MEM_opc = 4w \/ s'.MEM.MEM_opc = 5w \/
-                                                          s'.MEM.MEM_opc = 6w \/ s'.MEM.MEM_opc = 7w \/
-                                                          s'.MEM.MEM_opc = 8w \/ s'.MEM.MEM_opc = 9w \/
-                                                          s'.MEM.MEM_opc = 13w \/ s'.MEM.MEM_opc = 14w) in
-                                                                                    
-      s' with MEM := s'.MEM with MEM_isInterrupt := (s'.MEM.MEM_opc = 12w)
+  MEM_ctrl_update (fext:ext) s s' =
+  if (s.EX.EX_write_enable /\ s.MEM.MEM_state_flag) \/ s.MEM.MEM_enable then
+    let s' = s' with MEM := s'.MEM with MEM_read_mem := (s.MEM.MEM_opc = 4w \/ s.MEM.MEM_opc = 5w);
+        s' = s' with MEM := s'.MEM with MEM_write_mem := (s.MEM.MEM_opc = 2w);
+        s' = s' with MEM := s'.MEM with MEM_write_mem_byte := (s.MEM.MEM_opc = 3w) in
+      s' with MEM := s'.MEM with MEM_isInterrupt := (s.MEM.MEM_opc = 12w)
   else s'
 End
 
 (** generate the value for the LoadUpperConstant instruction **)
 Definition MEM_imm_update_def:
-  MEM_imm_update (fext:ext) (s:state_circuit) s' =
-  s' with MEM := s'.MEM with MEM_imm_updated := MUX_21 (s'.MEM.MEM_opc = 14w) s'.MEM.MEM_imm
+  MEM_imm_update (fext:ext) s s' =
+  s' with MEM := s'.MEM with MEM_imm_updated := MUX_21 (s.MEM.MEM_opc = 14w) s'.MEM.MEM_imm
                                                 ((8 >< 0) s'.MEM.MEM_imm @@ (22 >< 0) s'.MEM.MEM_dataW)
 End
 
 Theorem MEM_imm_update_trans = REWRITE_RULE [MUX_21_def] MEM_imm_update_def
 
-(** set up flags for WB stage **)
-Definition WB_ctrl_update_def:
-  WB_ctrl_update (fext:ext) (s:state_circuit) s' =
-  if (s'.MEM.MEM_write_enable /\ s'.WB.WB_state_flag) \/ s'.WB.WB_enable then
-    let s' = s' with WB := s'.WB with WB_isOut := (s'.WB.WB_opc = 6w) in
-      s' with WB := s'.WB with WB_data_sel := if s'.WB.WB_opc = 0w \/ s'.WB.WB_opc = 6w then 0w
-                                              else if s'.WB.WB_opc = 1w then 1w
-                                              else if s'.WB.WB_opc = 7w then 2w
-                                              else if s'.WB.WB_opc = 9w then 3w
-                                              else if s'.WB.WB_opc = 13w \/ s'.WB.WB_opc = 14w then 4w
-                                              else if s'.WB.WB_opc = 4w then 5w
-                                              else if s'.WB.WB_opc = 5w then 6w
-                                              else if s'.WB.WB_opc = 8w then 7w
-                                              else 0w
-  else s'
-End
-
-(** generate read data for the LoadMemByte instruction **)
-Definition WB_read_data_byte_update_def:
-  WB_read_data_byte_update (fext:ext) (s:state_circuit) s' =
-  s' with WB := s'.WB with WB_read_data_byte := MUX_41 ((1 >< 0) s'.WB.WB_dataA)
-                                                       (w2w ((7 >< 0) s'.WB.WB_read_data))
-                                                       (w2w ((15 >< 8) s'.WB.WB_read_data))
-                                                       (w2w ((23 >< 16) s'.WB.WB_read_data))
-                                                       (w2w ((31 >< 24) s'.WB.WB_read_data))
-End
-
-Theorem WB_read_data_byte_update_trans = REWRITE_RULE [MUX_41_def] WB_read_data_byte_update_def
-
-(** choose correct data based on WB_data_sel to write register **)
-Definition WB_write_data_update_def:
-  WB_write_data_update fext s s' =
-  s' with WB := s'.WB with WB_write_data := MUX_81 s'.WB.WB_data_sel s'.WB.WB_ALU_res
+(** update components for WB stage **)
+Definition WB_update_def:
+  WB_update fext (s:state_circuit) s' =
+  let s' = s' with WB := s'.WB with WB_read_data := fext.data_rdata;
+      s' = s' with WB := s'.WB with WB_read_data_byte := MUX_41 ((1 >< 0) s'.WB.WB_dataA)
+                                                                (w2w ((7 >< 0) s'.WB.WB_read_data))
+                                                                (w2w ((15 >< 8) s'.WB.WB_read_data))
+                                                                (w2w ((23 >< 16) s'.WB.WB_read_data))
+                                                                (w2w ((31 >< 24) s'.WB.WB_read_data));
+      s' = (if (s.MEM.MEM_write_enable /\ s.WB.WB_state_flag) \/ s.WB.WB_enable then
+              let s' = s' with WB := s'.WB with WB_isOut := (s'.WB.WB_opc = 6w) in
+                s' with WB := s'.WB with WB_data_sel :=
+                if s'.WB.WB_opc = 0w \/ s'.WB.WB_opc = 6w then 0w
+                else if s'.WB.WB_opc = 1w then 1w
+                else if s'.WB.WB_opc = 7w then 2w
+                else if s'.WB.WB_opc = 9w then 3w
+                else if s'.WB.WB_opc = 13w \/ s'.WB.WB_opc = 14w then 4w
+                else if s'.WB.WB_opc = 4w then 5w
+                else if s'.WB.WB_opc = 5w then 6w
+                else if s'.WB.WB_opc = 8w then 7w
+                else 0w
+            else s') in
+     s' with WB := s'.WB with WB_write_data := MUX_81 s'.WB.WB_data_sel s'.WB.WB_ALU_res
                                                    s'.WB.WB_SHIFT_res (w2w fext.data_in)
                                                    (s'.WB.WB_PC + 4w) s'.WB.WB_imm
                                                    s'.WB.WB_read_data s'.WB.WB_read_data_byte
-                                                   s.acc_res
+                                                   s.acc_res                      
 End
 
-Theorem WB_write_data_update_trans = REWRITE_RULE [MUX_81_def] WB_write_data_update_def
+Theorem WB_update_trans = REWRITE_RULE [MUX_81_def,MUX_41_def] WB_update_def
 
 (** hazard handling **)
 Definition Hazard_ctrl_def:
-  Hazard_ctrl fext (s:state_circuit) s' =
+  Hazard_ctrl fext s s' =
   if s'.state = 3w \/ s'.state = 5w then
     let s' = s' with IF := s'.IF with IF_PC_write_enable := F;
         s' = s' with ID := s'.ID with ID_ID_write_enable := F;
@@ -399,8 +358,8 @@ Definition Hazard_ctrl_def:
         s' = s' with MEM := s'.MEM with MEM_state_flag := F;
         s' = s' with MEM := s'.MEM with MEM_NOP_flag := F in
     s' with WB := s'.WB with WB_state_flag := F
-  else if s'.MEM.MEM_opc = 2w \/ s'.MEM.MEM_opc = 3w \/ s'.MEM.MEM_opc = 4w \/
-          s'.MEM.MEM_opc = 5w \/ s'.MEM.MEM_opc = 12w then
+  else if s.MEM.MEM_opc = 2w \/ s.MEM.MEM_opc = 3w \/ s.MEM.MEM_opc = 4w \/
+          s.MEM.MEM_opc = 5w \/ s.MEM.MEM_opc = 12w then
     let s' = s' with IF := s'.IF with IF_PC_write_enable := F;
         s' = s' with ID := s'.ID with ID_ID_write_enable := F;
         s' = s' with ID := s'.ID with ID_flush_flag := F;
@@ -409,7 +368,7 @@ Definition Hazard_ctrl_def:
         s' = s' with MEM := s'.MEM with MEM_state_flag := F;
         s' = s' with MEM := s'.MEM with MEM_NOP_flag := T in
     s' with WB := s'.WB with WB_state_flag := T
-  else if s'.IF.PC_sel <> 0w then
+  else if s.IF.PC_sel <> 0w then
     let s' = s' with IF := s'.IF with IF_PC_write_enable := T;
         s' = s' with ID := s'.ID with ID_ID_write_enable := F;
         s' = s' with ID := s'.ID with ID_flush_flag := T;
@@ -431,55 +390,50 @@ End
 
 (** data forwarding **)
 Definition Forward_update_def:
-  Forward_update EX_addr addr_disable check s : word3 =
-  if EX_addr = s.MEM.MEM_addrW /\ s.MEM.MEM_write_reg /\
+  Forward_update EX_addr addr_disable check s s' : word3 =
+  if EX_addr = s.MEM.MEM_addrW /\ s'.MEM.MEM_write_reg /\
      (s.MEM.MEM_opc = 13w \/ s.MEM.MEM_opc = 14w) /\ (~ addr_disable) /\ check then 5w
-  else if EX_addr = s.MEM.MEM_addrW /\ s.MEM.MEM_write_reg /\
+  else if EX_addr = s.MEM.MEM_addrW /\ s'.MEM.MEM_write_reg /\
           s.MEM.MEM_opc = 9w /\ (~ addr_disable) /\ check then 4w
-  else if EX_addr = s.MEM.MEM_addrW /\ s.MEM.MEM_write_reg /\
+  else if EX_addr = s.MEM.MEM_addrW /\ s'.MEM.MEM_write_reg /\
           s.MEM.MEM_opc = 1w /\ (~ addr_disable) /\ check then 3w
-  else if EX_addr = s.MEM.MEM_addrW /\ s.MEM.MEM_write_reg /\
+  else if EX_addr = s.MEM.MEM_addrW /\ s'.MEM.MEM_write_reg /\
           (s.MEM.MEM_opc = 0w \/ s.MEM.MEM_opc = 6w) /\ (~ addr_disable) /\ check then 2w
   else if EX_addr = s.WB.WB_addrW /\ s.WB.WB_write_reg /\ (~ addr_disable) /\ check then 1w
   else 0w
 End
 
 Definition ForwardA_def:
-  ForwardA (fext:ext) (s:state_circuit) s' =
-  let checkA = (s'.EX.EX_opc = 0w \/ s'.EX.EX_opc = 1w \/ s'.EX.EX_opc = 2w \/ s'.EX.EX_opc = 3w \/
-                s'.EX.EX_opc = 4w \/ s'.EX.EX_opc = 5w \/ s'.EX.EX_opc = 6w \/ s'.EX.EX_opc = 8w \/
-                s'.EX.EX_opc = 9w \/ s'.EX.EX_opc = 10w \/ s'.EX.EX_opc = 11w) in
+  ForwardA (fext:ext) s s' =
+  let s' = s' with checkA :=
+           (s.EX.EX_opc = 0w \/ s.EX.EX_opc = 1w \/ s.EX.EX_opc = 2w \/ s.EX.EX_opc = 3w \/
+            s.EX.EX_opc = 4w \/ s.EX.EX_opc = 5w \/ s.EX.EX_opc = 6w \/ s.EX.EX_opc = 8w \/
+            s.EX.EX_opc = 9w \/ s.EX.EX_opc = 10w \/ s.EX.EX_opc = 11w) in
     s' with EX := s'.EX with EX_ForwardA :=
-    Forward_update s'.EX.EX_addrA s'.EX.EX_addrA_enable checkA s'
+    Forward_update s'.EX.EX_addrA s'.EX.EX_addrA_enable s'.checkA s s'
 End
 
 Theorem ForwardA_trans = REWRITE_RULE [Forward_update_def] ForwardA_def
 
 Definition ForwardB_def:
-  ForwardB (fext:ext) (s:state_circuit) s' =
-  let checkB = (s'.EX.EX_opc = 0w \/ s'.EX.EX_opc = 1w \/ s'.EX.EX_opc = 2w \/ s'.EX.EX_opc = 3w \/
-                s'.EX.EX_opc = 6w \/ s'.EX.EX_opc = 10w \/ s'.EX.EX_opc = 11w) in
+  ForwardB (fext:ext) s s' =
+  let s' = s' with checkB :=
+           (s.EX.EX_opc = 0w \/ s.EX.EX_opc = 1w \/ s.EX.EX_opc = 2w \/ s.EX.EX_opc = 3w \/
+            s.EX.EX_opc = 6w \/ s.EX.EX_opc = 10w \/ s.EX.EX_opc = 11w) in
     s' with EX := s'.EX with EX_ForwardB :=
-    Forward_update s'.EX.EX_addrB s'.EX.EX_addrB_enable checkB s'
+    Forward_update s'.EX.EX_addrB s'.EX.EX_addrB_enable s'.checkB s s'
 End
 
 Theorem ForwardB_trans = REWRITE_RULE [Forward_update_def] ForwardB_def
                                        
 Definition ForwardW_def:
-  ForwardW (fext:ext) (s:state_circuit) s' =
-  let checkW = (s'.EX.EX_opc = 10w \/ s'.EX.EX_opc = 11w \/ s'.EX.EX_opc = 14w) in
+  ForwardW (fext:ext) s s' =
+  let s' = s' with checkW := (s.EX.EX_opc = 10w \/ s.EX.EX_opc = 11w \/ s.EX.EX_opc = 14w) in
     s' with EX := s'.EX with EX_ForwardW :=
-    Forward_update s'.EX.EX_addrW s'.EX.EX_addrW_enable checkW s'
+    Forward_update s.EX.EX_addrW s'.EX.EX_addrW_enable s'.checkW s s'
 End
 
 Theorem ForwardW_trans = REWRITE_RULE [Forward_update_def] ForwardW_def
-
-(** assign some items **)
-Definition assign_update_def:
-  assign_update fext (s:state_circuit) s' =
-  let s' = s' with IF := s'.IF with IF_instr := if fext.ready then fext.inst_rdata else 0x0000003Fw in
-    s' with WB := s'.WB with WB_read_data := fext.data_rdata
-End
 
 
 (* always_ff related: triggered by posedge clk *)
@@ -493,9 +447,9 @@ End
 
 (** decode: IF -> ID **)
 Definition ID_pipeline_def:
-  ID_pipeline (fext:ext) (s:state_circuit) s' =
+  ID_pipeline (fext:ext) s s' =
   if s'.ID.ID_ID_write_enable then
-    let s' = s' with ID := s'.ID with ID_PC := s'.PC in
+    let s' = s' with ID := s'.ID with ID_PC := s.PC in
     s' with ID := s'.ID with ID_instr := s'.IF.IF_instr
   else if s'.ID.ID_flush_flag then
     s' with ID := s'.ID with ID_instr := 0x0000003Fw
@@ -504,17 +458,17 @@ End
 
 (** register write **)
 Definition REG_write_def:
-  REG_write (fext:ext) (s:state_circuit) s' =
-  if s'.WB.WB_write_reg /\ s'.WB.WB_state_flag then
-    s' with R := (s'.WB.WB_addrW =+ s'.WB.WB_write_data) s'.R
+  REG_write (fext:ext) s s' =
+  if s.WB.WB_write_reg /\ s.WB.WB_state_flag then
+    s' with R := (s.WB.WB_addrW =+ s.WB.WB_write_data) s'.R
   else s'
 End
 
 (** execute: ID -> EX **)
 Definition EX_pipeline_def:
-  EX_pipeline (fext:ext) (s:state_circuit) s' =
-  if s'.ID.ID_EX_write_enable then
-    let s' = s' with EX := s'.EX with EX_PC := s'.ID.ID_PC;
+  EX_pipeline (fext:ext) s s' =
+  if s.ID.ID_EX_write_enable then
+    let s' = s' with EX := s'.EX with EX_PC := s.ID.ID_PC;
         s' = s' with EX := s'.EX with EX_dataA := s'.ID.ID_dataA;
         s' = s' with EX := s'.EX with EX_dataB := s'.ID.ID_dataB;
         s' = s' with EX := s'.EX with EX_dataW := s'.ID.ID_dataW;
@@ -526,46 +480,54 @@ Definition EX_pipeline_def:
         s' = s' with EX := s'.EX with EX_addrA := s'.ID.ID_addrA;
         s' = s' with EX := s'.EX with EX_addrB := s'.ID.ID_addrB;
         s' = s' with EX := s'.EX with EX_addrW := s'.ID.ID_addrW;
-        s' = s' with EX := s'.EX with EX_opc := if s'.EX.EX_NOP_flag then 16w else s'.ID.ID_opc;
-        s' = s' with EX := s'.EX with EX_func := s'.ID.ID_func in
-      s' with EX := s'.EX with EX_PC_sel := if s'.ID.ID_opc = 9w then 1w
-                                            else if s'.ID.ID_opc = 10w then 2w
-                                            else if s'.ID.ID_opc = 11w then 3w
-                                            else 0w
+        s' = s' with EX := s'.EX with EX_opc := if s'.EX.EX_NOP_flag then 16w else s'.ID.ID_opc in
+      s' with EX := s'.EX with EX_func := s'.ID.ID_func
   else
     s' with EX := s'.EX with EX_write_enable := F
 End
 
 (** memory: EX -> MEM **)
 Definition MEM_pipeline_def:
-  MEM_pipeline (fext:ext) (s:state_circuit) s' =
-  if (s'.EX.EX_write_enable /\ s'.MEM.MEM_state_flag) \/ s'.MEM.MEM_enable then
-    let s' = s' with MEM := s'.MEM with MEM_PC := s'.EX.EX_PC;
-        s' = s' with MEM := s'.MEM with MEM_dataA := s'.EX.EX_dataA_rec;
-        s' = s' with MEM := s'.MEM with MEM_dataB := s'.EX.EX_dataB_rec;
-        s' = s' with MEM := s'.MEM with MEM_dataW := s'.EX.EX_dataW_rec;
-        s' = s' with MEM := s'.MEM with MEM_imm := s'.EX.EX_imm;
-        s' = s' with MEM := s'.MEM with MEM_ALU_res := s'.EX.EX_ALU_res;
-        s' = s' with MEM := s'.MEM with MEM_SHIFT_res := s'.EX.EX_SHIFT_res;
-        s' = s' with MEM := s'.MEM with MEM_write_enable := T;
-        s' = s' with MEM := s'.MEM with MEM_addrW := s'.EX.EX_addrW in
-      s' with MEM := s'.MEM with MEM_opc := if s'.MEM.MEM_NOP_flag then 16w else s'.EX.EX_opc
-  else
-    s' with MEM := s'.MEM with MEM_write_enable := F
+  MEM_pipeline (fext:ext) s s' =
+  let s' = (if (s.EX.EX_write_enable /\ s.MEM.MEM_state_flag) \/ s.MEM.MEM_enable then
+              let s' = s' with MEM := s'.MEM with MEM_PC := s.EX.EX_PC;
+                  s' = s' with MEM := s'.MEM with MEM_dataA := s'.EX.EX_dataA_rec;
+                  s' = s' with MEM := s'.MEM with MEM_dataB := s'.EX.EX_dataB_rec;
+                  s' = s' with MEM := s'.MEM with MEM_dataW := s'.EX.EX_dataW_rec;
+                  s' = s' with MEM := s'.MEM with MEM_imm := s.EX.EX_imm;
+                  s' = s' with MEM := s'.MEM with MEM_ALU_res := s'.EX.EX_ALU_res;
+                  s' = s' with MEM := s'.MEM with MEM_SHIFT_res := s'.EX.EX_SHIFT_res;
+                  s' = s' with MEM := s'.MEM with MEM_write_enable := T;
+                  s' = s' with MEM := s'.MEM with MEM_addrW := s.EX.EX_addrW;
+                  s' = s' with MEM := s'.MEM with MEM_opc := s.EX.EX_opc in
+                s' with MEM := s'.MEM with MEM_write_reg :=
+                ((s.EX.EX_opc = 0w) \/ (s.EX.EX_opc = 1w) \/ (s.EX.EX_opc = 4w) \/
+                (s.EX.EX_opc = 5w) \/ (s.EX.EX_opc = 6w) \/ (s.EX.EX_opc = 7w) \/
+                (s.EX.EX_opc = 8w) \/ (s.EX.EX_opc = 9w) \/ (s.EX.EX_opc = 13w) \/
+                (s.EX.EX_opc = 14w))
+            else
+              s' with MEM := s'.MEM with MEM_write_enable := F) in
+    if s'.MEM.MEM_NOP_flag then
+      s' with MEM := s'.MEM with MEM_opc := 16w
+    else s'
 End
 
 (** write back: MEM -> WB **)
 Definition WB_pipeline_def:
-  WB_pipeline (fext:ext) (s:state_circuit) s' =
-  if (s'.MEM.MEM_write_enable /\ s'.WB.WB_state_flag) \/ s'.WB.WB_enable then
-    let s' = s' with WB := s'.WB with WB_PC := s'.MEM.MEM_PC;
-        s' = s' with WB := s'.WB with WB_dataA := s'.MEM.MEM_dataA;
-        s' = s' with WB := s'.WB with WB_imm := s'.MEM.MEM_imm;
-        s' = s' with WB := s'.WB with WB_ALU_res := s'.MEM.MEM_ALU_res;
-        s' = s' with WB := s'.WB with WB_SHIFT_res := s'.MEM.MEM_SHIFT_res;
-        s' = s' with WB := s'.WB with WB_write_reg := s'.MEM.MEM_write_reg;
-        s' = s' with WB := s'.WB with WB_addrW := s'.MEM.MEM_addrW in
-      s' with WB := s'.WB with WB_opc := s'.MEM.MEM_opc
+  WB_pipeline (fext:ext) s s' =
+  if (s.MEM.MEM_write_enable /\ s.WB.WB_state_flag) \/ s.WB.WB_enable then
+    let s' = s' with WB := s'.WB with WB_PC := s.MEM.MEM_PC;
+        s' = s' with WB := s'.WB with WB_dataA := s.MEM.MEM_dataA;
+        s' = s' with WB := s'.WB with WB_imm := s.MEM.MEM_imm_updated;
+        s' = s' with WB := s'.WB with WB_ALU_res := s.MEM.MEM_ALU_res;
+        s' = s' with WB := s'.WB with WB_SHIFT_res := s.MEM.MEM_SHIFT_res;
+        s' = s' with WB := s'.WB with WB_write_reg :=
+             ((s.MEM.MEM_opc = 0w) \/ (s.MEM.MEM_opc = 1w) \/ (s.MEM.MEM_opc = 4w) \/
+             (s.MEM.MEM_opc = 5w) \/ (s.MEM.MEM_opc = 6w) \/ (s.MEM.MEM_opc = 7w) \/
+             (s.MEM.MEM_opc = 8w) \/ (s.MEM.MEM_opc = 9w) \/ (s.MEM.MEM_opc = 13w) \/
+             (s.MEM.MEM_opc = 14w));
+        s' = s' with WB := s'.WB with WB_addrW := s.MEM.MEM_addrW in
+      s' with WB := s'.WB with WB_opc := s.MEM.MEM_opc
   else s'
 End
 
@@ -587,30 +549,30 @@ Definition agp32_next_state_def:
               else if s'.MEM.MEM_read_mem then
                 let s' = s' with state := 7w;
                     s' = s' with command := 2w in
-                  s' with data_addr := s'.MEM.MEM_dataA
+                  s' with data_addr := s.MEM.MEM_dataA
               else if s'.MEM.MEM_write_mem then
                 let s' = s' with state := 7w;
                     s' = s' with command := 3w;
-                    s' = s' with data_addr := s'.MEM.MEM_dataB;
-                    s' = s' with data_wdata := s'.MEM.MEM_dataA in
+                    s' = s' with data_addr := s.MEM.MEM_dataB;
+                    s' = s' with data_wdata := s.MEM.MEM_dataA in
                   s' with data_wstrb := 15w
               else if s'.MEM.MEM_write_mem_byte then
                 let s' = s' with state := 7w;
                     s' = s' with command := 3w;
-                    s' = s' with data_addr := s'.MEM.MEM_dataB;
-                    s' = s' with data_wstrb := 1w <<~ w2w ((1 >< 0) s'.MEM.MEM_dataB) in
-               case (1 >< 0) s'.MEM.MEM_dataB of
-                 0w => s' with data_wdata := bit_field_insert 7 0 ((7 >< 0) s'.MEM.MEM_dataA) s'.data_wdata
-               | 1w => s' with data_wdata := bit_field_insert 15 8 ((7 >< 0) s'.MEM.MEM_dataA) s'.data_wdata
-               | 2w => s' with data_wdata := bit_field_insert 23 16 ((7 >< 0) s'.MEM.MEM_dataA) s'.data_wdata
-               | 3w => s' with data_wdata := bit_field_insert 31 24 ((7 >< 0) s'.MEM.MEM_dataA) s'.data_wdata
-              else if (s'.IF.PC_sel <> 0w) then
+                    s' = s' with data_addr := s.MEM.MEM_dataB;
+                    s' = s' with data_wstrb := 1w <<~ w2w ((1 >< 0) s.MEM.MEM_dataB) in
+               case (1 >< 0) s.MEM.MEM_dataB of
+                 0w => s' with data_wdata := bit_field_insert 7 0 ((7 >< 0) s.MEM.MEM_dataA) s'.data_wdata
+               | 1w => s' with data_wdata := bit_field_insert 15 8 ((7 >< 0) s.MEM.MEM_dataA) s'.data_wdata
+               | 2w => s' with data_wdata := bit_field_insert 23 16 ((7 >< 0) s.MEM.MEM_dataA) s'.data_wdata
+               | 3w => s' with data_wdata := bit_field_insert 31 24 ((7 >< 0) s.MEM.MEM_dataA) s'.data_wdata
+              else if (s.IF.PC_sel <> 0w) then
                 let s' = s' with state := 1w in
                   s' with command := 1w
               else if s'.EX.EX_isAcc then
                 let s' = s' with state := 2w;
                     s' = s' with command := 0w;
-                s' = s' with acc_arg := s'.EX.EX_dataA_updated in
+                s' = s' with acc_arg := s.EX.EX_dataA_updated in
                   s' with acc_arg_ready := T
               else s')
     | 1w => (let s' = if fext.ready /\ s.command = 0w then s' with state := 6w           
@@ -675,8 +637,8 @@ val init_tm = add_x_inits ``<| R := K 0w;
                                ID := <| ID_instr := 0x0000003Fw; ID_ForwardA := F;                   
                                         ID_ForwardB := F; ID_ForwardW := F |>;
                                EX := <| EX_ForwardA := 0w; EX_ForwardB := 0w; EX_ForwardW := 0w;
-                                        EX_PC_sel := 0w |>;
-                               MEM := <| MEM_enable := F |>;                              
+                                        EX_PC_sel := 0w; EX_opc := 15w |>;
+                               MEM := <| MEM_enable := F; MEM_write_reg := F; MEM_opc := 15w |>;
                                WB := <| WB_enable := F; WB_write_reg := F |> |>``;
 
 Definition agp32_init_def:
@@ -685,17 +647,14 @@ End
 
 (** pipelined Silver **)
 Definition agp32_def:
-  agp32 = mk_module (procs [IF_PC_update; ID_pipeline; REG_write; EX_pipeline;
-                            MEM_pipeline; WB_pipeline; agp32_next_state; Acc_compute])
-                    (procs [IF_PC_sel_update; IF_PC_input_update; ID_addr_update;
-                            ID_opc_update; ID_func_update; REG_read; ID_imm_update;
-                            ID_imm_reg_update; ID_forward_update; ID_read_data_update;
-                            ID_data_update; EX_ctrl_update; EX_forward_data;
-                            EX_ALU_input_update; EX_compute_enable_update;
-                            EX_ALU_update; EX_SHIFT_update; EX_data_rec_update;
-                            MEM_ctrl_update; MEM_imm_update; WB_ctrl_update;
-                            WB_read_data_byte_update; WB_write_data_update;
-                            Hazard_ctrl; ForwardA; ForwardB; ForwardW; assign_update])
+  agp32 = mk_module (procs [agp32_next_state; WB_pipeline; MEM_pipeline;
+                            EX_pipeline; REG_write; ID_pipeline; IF_PC_update; Acc_compute])
+                    (procs [WB_update; MEM_imm_update; MEM_ctrl_update; EX_data_rec_update;
+                            EX_SHIFT_update; EX_ALU_update; EX_compute_enable_update;
+                            EX_ALU_input_update; EX_forward_data; EX_ctrl_update;
+                            ID_data_update; ID_imm_update; ID_opc_func_update;
+                            IF_PC_input_update; ForwardW; ForwardB; ForwardA;
+                            Hazard_ctrl; IF_PC_sel_update; IF_instr_update])
                     agp32_init
 End
 
